
Concepts

Measurement outcomes
set of all possible measurement outcomes with respect to the grid cell C of all laser scans𝐴

𝑧
𝑧'

that are recorded close enough to potentially measure the cell. These measurement outcomes
will be used for computing the entropy and the mutual information between the map and each
cell.

Measurement outcomes is a set of three values obtained from the proposed inverse𝑧'
measurement model . After a new laser measurement is received, all the cells that[𝑙
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can be seen are found, then we apply the inverse measurement model to obtain the set of three
values stated above.

The number of measurement outcomes is given by the number of ways to sample k elements
from the set of 3 laser measurement outcomes with replacement and disregarding[𝑙
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different ordering. For calculating the number of combinations use the equation (3.13 from the
Thesis or 12 from the paper). The explanation in the paper is better for this point.

Outcomes probabilities
Algorithm 1 computes the probabilities of the outcomes by propagating the probability mass
through the graph, for this, the algorithm uses a hash table P(<-, -, ->) which is indexed by the
measurement histograms.

Measurement histograms
This one is the possible combinations based on all the available measurements, the order is not
important in this case.

Notes
The outcome probabilities from my understanding are the probabilities produced by propagating
the probabilities of the current reading to the next one (Even if there are no more readings), for
example we have two measurements that saw a cell (Level 2), then we will propagate the
probabilities for the next level (Which is proposed by the algorithm). Looking at the algorithm it
starts in one of the cells that fulfills the condition f + o + u = r, and from that point we calculate
the probability of the next level based on the current measurement outcomes and probabilities.
See the left hand side of the Figure 3.4, probabilities are calculated in that way; however in the
right hand side we have the representation of all the measurement outcomes (In this case𝑧'



replacement takes place so we have a reduction in the number of combinations, this is
equivalent to different combinations).



Algorithm test
This is my interpretation.

Testing with a set of two measurements (k = 2) for a specific cell (The cell is not relevant at all)

<f, o, u> that fulfills. f + o + u = 1
Using 3.13 we get 3 (Three possible different results)
Using 3.14 we get 9 (All possible probabilities)
<1, 0, 0>, <0, 1, 0>, <0, 0, 1>

Loop for r = 1
Taking: <1, 0, 0>

P(<2, 0, 0>) += P(<1, 0, 0>) * P( observes C as free);𝑍
𝑖
𝑗

P(<1, 1, 0>) += P(<1, 0, 0>) * P( observes C as occupied); - Adding𝑍
𝑖
𝑗

P(<1, 0, 1>) += P(<1, 0, 0>) * P( does not observe C); - Adding𝑍
𝑖
𝑗

Taking: <0, 1, 0>

P(<1, 1, 0>) += P(<0, 1, 0>) * P( observes C as free); - Adding𝑍
𝑖
𝑗

P(<0, 2, 0>) += P(<0, 1, 0>) * P( observes C as occupied);𝑍
𝑖
𝑗

P(<0, 1, 1>) += P(<0, 1, 0>) * P( does not observe C); - Adding𝑍
𝑖
𝑗

Taking: <0, 0, 1>

P(<1, 0, 1>) += P(<0, 0, 1>) * P( observes C as free); - Adding𝑍
𝑖
𝑗

P(<0, 1, 1>) += P(<0, 0, 1>) * P( observes C as occupied); - Adding𝑍
𝑖
𝑗

P(<0, 0, 2>) += P(<0, 0, 1>) * P( does not observe C);𝑍
𝑖
𝑗

<f, o, u> that fulfills. f + o + u = 2
Using 3.13 we get 6 (Three possible different results). These were filled before in the loop when
r = 1
Using 3.14 we get 36 (All possible probabilities) - There is an incongruity in this equation. On
the left side we got 27 and on the right side of the equation we got 36). Also note that the 36 is
the total computation of probabilities including the ones at the first step.
<2, 0, 0>, <1, 1, 0>, <0, 2, 0>, <0, 1, 1>, <1, 0, 1>, <0, 0, 2>



Loop for r = 2
Using 3.13 we get 6 (Six possible different results). T
Taking: <2, 0, 0>

P(<3, 0, 0>) += P(<2, 0, 0>) * P( observes C as free); - 1𝑍
𝑖
𝑗

P(<2, 1, 0>) += P(<2, 0, 0>) * P( observes C as occupied); - Adding - 2𝑍
𝑖
𝑗

P(<2, 0, 1>) += P(<2, 0, 0>) * P( does not observe C); - Adding - 3𝑍
𝑖
𝑗

Taking: <1, 1, 0>

P(<2, 1, 0>) += P(<1, 1, 0>) * P( observes C as free); - Adding𝑍
𝑖
𝑗

P(<1, 2, 0>) += P(<1, 1, 0>) * P( observes C as occupied); - Adding - 4𝑍
𝑖
𝑗

P(<1, 1, 1>) += P(<1, 1, 0>) * P( does not observe C); - Adding - 5𝑍
𝑖
𝑗

Taking: <0, 2, 0>

P(<1, 2, 0>) += P(<0, 2, 0>) * P( observes C as free); - Adding𝑍
𝑖
𝑗

P(<0, 3, 0>) += P(<0, 2, 0>) * P( observes C as occupied); - 6𝑍
𝑖
𝑗

P(<0, 2, 1>) += P(<0, 2, 0>) * P( does not observe C); - Adding - 7𝑍
𝑖
𝑗

Taking: <0, 1, 1>

P(<1, 1, 1>) += P(<0, 1, 1>) * P( observes C as free); - Adding𝑍
𝑖
𝑗

P(<0, 2, 1>) += P(<0, 1, 1>) * P( observes C as occupied); - Adding𝑍
𝑖
𝑗

P(<0, 1, 2>) += P(<0, 1, 1>) * P( does not observe C); - Adding - 8𝑍
𝑖
𝑗

Taking: <1, 0, 1>

P(<2, 0, 1>) += P(<1, 0, 1>) * P( observes C as free); - Adding𝑍
𝑖
𝑗

P(<1, 1, 1>) += P(<1, 0, 1>) * P( observes C as occupied); - Adding𝑍
𝑖
𝑗

P(<1, 0, 2>) += P(<1, 0, 1>) * P( does not observe C); - Adding - 9𝑍
𝑖
𝑗

Taking: <0, 0, 2>

P(<1, 0, 2>) += P(<0, 0, 2>) * P( observes C as free); - Adding𝑍
𝑖
𝑗

P(<0, 1, 2>) += P(<0, 0, 2>) * P( observes C as occupied); - Adding𝑍
𝑖
𝑗

P(<0, 0, 3>) += P(<0, 0, 2>) * P( does not observe C); - 10𝑍
𝑖
𝑗



Algorithm
Algorithm input: Set of k laser measurements Z, cell C
Algorithm output: Probabilities P(<-, -, ->) of the outcomes (free, occupied, not observed)
Initial condition: P(<0, 0, 0>) = 1 (This is the root of the graph)
Loop
for r=1 .. k do

for all <f, o, u> with f + o + u == r do
P(<f + 1, o , u>) += P(<f, u, o>)*P( observes C as free);𝑍

𝑖
𝑗

P(<f, o + 1 , u>) += P(<f, u, o>)*P( observes C as occupied);𝑍
𝑖
𝑗

P(<f , o , u + 1>) += P(<f, u, o>)*P( does not observe C);𝑍
𝑖
𝑗

end for
end for
return P(<-, -, ->)


